{
 "cells": [
  {
   "cell_type": "code",
   "execution_count": null,
   "id": "937616f1-1dfd-41fb-88f4-f7cffb5cea36",
   "metadata": {},
   "outputs": [],
   "source": [
    "1. Find the value of T(2) for the recurrence relation T(n) = 3T(n-1) + 12n, given that T(0)=5.\n",
    "\n",
    "T(n) = 3T(n-1) + 12n\n",
    "\n",
    "We know that for n=0, T(0)=5\n",
    "Therefore we put n-1=0 => n=1\n",
    "\n",
    "T(1) = 3T(1-1) + 12x1 = 3T(0) + 12 = 3 x 5 + 12 = 27\n",
    "T(2) = 3T(2-1) + 12x2 = 3T(1) + 24 = 3 x 27 + 24 = 105\n",
    "\n",
    "T(2) = 105"
   ]
  },
  {
   "cell_type": "code",
   "execution_count": null,
   "id": "1873ba78-a9cf-4ba6-8ec1-f47c6fb16eb8",
   "metadata": {},
   "outputs": [],
   "source": [
    "2. Given a recurrence relation, solve it using substitution method\n",
    "\n",
    "a. T(n) = T(n-1)+c ------ 1\n",
    "\n",
    "Substitute n with n-1\n",
    "\n",
    "T(n-1) = T(n-2)+c ------- 2\n",
    "\n",
    "Continuing the substitution one more time\n",
    "\n",
    "T(n-2) = T(n-3)+c ------- 3\n",
    "\n",
    "Replace equation 2 in equation 1\n",
    "\n",
    "T(n) = T(n-2)+2c -------- 4\n",
    "\n",
    "Replace equation 4 in equation 3, \n",
    "T(n) = T(n-3) + 3c\n",
    "\n",
    "Continuing substitution k number of times,\n",
    "T(n) = T(n-k) + kc\n",
    "\n",
    "Considering the base case condition, when n-1, T(n) becomes 1.\n",
    "\n",
    "Therefore we make n-k=1, so that T(n-k) becomes 1\n",
    "\n",
    "n-k=1 => k=n-1\n",
    "\n",
    "T(n) = T(n-(n-1))+(n-1)c\n",
    "     = T(n-n+1)+(n-1)c\n",
    "     = T(1) + nc - c\n",
    "     = 1+nc-c\n",
    "     \n",
    "After eradicating the constant value, T(n)=O(n)\n",
    "\n",
    "\n",
    "\n",
    "b. T(n) = 2T(n/2) + n ------------- 1\n",
    "\n",
    "Substitue n with n/2\n",
    "T(n/2) = 2T(n/2^2) + n/2 --------- 2\n",
    "\n",
    "Substitute n with n/2 further,\n",
    "T(n/2^2) = 2T(n/2^3) + n/2^2 ----- 3\n",
    "\n",
    "Replace equation 2 in equation 1,\n",
    "T(n) = 2(2T(n/2^2) + n/2) + n\n",
    "     = 4T(n/2^2) + 2n ----------- 4\n",
    "     \n",
    "Replace equation 3 in equation 4\n",
    "\n",
    "T(n) = 4(2T(n/2^3) + n/2^2) + 2n\n",
    "     = 2^3 x T(n/2^3) + 3n\n",
    "     \n",
    "Continuing the substitution k times,\n",
    "T(n_ = 2^k T(n/2^k) + kn -------- 5\n",
    "\n",
    "Considering the base case condition, T(n/2^k) becomes 1 when n/2^k is equal to 1.\n",
    "\n",
    "Therefore n/2^k = 1 => n = 2^k => log2(n) = k log2(2) => k = log2(n)\n",
    "\n",
    "T(n) = 2^(log2(n)) T(n/2^(log2(n))) + n log2(n)\n",
    "     = 2^log2(n) T(1) + n log2(n)\n",
    "     = n^(log2(2)) + n^(log2(n))\n",
    "     = n + n log2(n)\n",
    "\n",
    "Therefore T(n) = O(n logn)\n",
    "\n",
    "  \n",
    "  \n",
    "c. T(n) = 2T(n/2) + c --------- 1\n",
    "  \n",
    "Substitute n with n/2\n",
    "  \n",
    "T(n/2) = 2T(n/2^2) + c -------- 2\n",
    "  \n",
    "Substitute n with n/2 further\n",
    "\n",
    "T(n/2^2) = 2T(n/2^3) + c -------- 3\n",
    "\n",
    "Replacing equation 2 in equation 1\n",
    "\n",
    "T(n) = 2(2T(n/2^2) + c) + c\n",
    "     = 4T(n/2^2) + 3c --------- 4\n",
    "     \n",
    "\n",
    "Replacing equation 3 in equation 4\n",
    "\n",
    "T(n) = 4(2T(n/2^3) + c) + 3c\n",
    "     = 8T(n/2^3) + 7c\n",
    "     = 2^3T(n/2^3) + (2^3-1) c -------- 5\n",
    "     \n",
    "\n",
    "Continuing the substitution k times,\n",
    "T(n) = 2^k T(n/2^k) + (2^k-1) c -------- 6\n",
    "\n",
    "When the value of n/2^k =1, the value of T(n/2^k) = 1.\n",
    "\n",
    "Hence deriving the value of k,\n",
    "n/2^k = 1 => log n = k log2(2) => k = log2(n)\n",
    "\n",
    "Substituting the value of k in equation 6\n",
    "\n",
    "T(n) = 2^k T(n/2^k) + (2^k-1)c\n",
    "     = 2^log2(n) T(n/2^log2(n)) + (2^log2(n) - 1) c\n",
    "     = n^log2(2) T(n/n^log2(2)) + (n^log2(2) - 1) c\n",
    "     = n T(1) + (n-1) c\n",
    "     = n + (n-1) c \n",
    " \n",
    "Therefore T(n) = O(n)\n",
    "  \n",
    "  \n",
    "d. T(n) = T(n/2) + c -------- 1\n",
    "\n",
    "Substitute n with n/2\n",
    "\n",
    "T(n/2) = T(n/2^2) + c ------ 2\n",
    "\n",
    "T(n/2^2) = T(n/2^3) + c ----- 3\n",
    "\n",
    "Replace equation 2 in equation 1\n",
    "\n",
    "T(n) = T(n/2^2) + 2c -------- 4\n",
    "\n",
    "Replace equation 3 in equation 4\n",
    "\n",
    "T(n) = T(n/2^3) + 3c -------- 5\n",
    "\n",
    "Continuing the substitution further upto k times\n",
    "\n",
    "T(n) = T(n/2^k) + kc -------- 6\n",
    "\n",
    "When n/2^k = 1, the entire T(n/2^k) attains the base case condition\n",
    "\n",
    "Therefore we make n/2^k = 1 => n=2^k => log2(n) = klog2(2) => k = log n\n",
    "\n",
    "\n",
    "Replacing k=log n in 6\n",
    "\n",
    "T(n)= T(n/2^log2(n)) + log2(n).c\n",
    "\n",
    "Using logarithmic property,\n",
    "T(n) = T(n/n^log2(2)) + log2(n).c\n",
    "     = T(n/n) + log2(n).c\n",
    "     = T(1) + log2(n).c\n",
    "     = c + log2(n).c\n",
    "     \n",
    "Eradicating the constant value,\n",
    "T(n) = O(log n)\n"
   ]
  },
  {
   "cell_type": "code",
   "execution_count": null,
   "id": "78fadc26-ce6d-4138-95ed-dff02ecc5d3e",
   "metadata": {},
   "outputs": [],
   "source": [
    "3. Given a recurrence relation, solve it using the recursive tree approach:\n",
    "\n",
    "\n",
    "a. T(n) = 2T(n-1) + 1\n",
    "T(n) = T(n-1) + T(n-1) + 1\n",
    "\n",
    "\n",
    "                n - 1 --- 2^0\n",
    "               / \\\n",
    "              /  \\\n",
    "             /    \\\n",
    "        1 - n-1   n-1 - 1 ---- 2^1\n",
    "           /|     /  \\\n",
    "          / |    /   \\\n",
    "    1 - n-2 n-2 n-2   n-2 - 1 ----- 2^2\n",
    "            \n",
    "\n",
    "Continuing till k times\n",
    "\n",
    "n-k = 0 (Base case condition)\n",
    "n=k\n",
    "\n",
    "T(n) = 1+2+4+8+..... 2^k\n",
    "     = 2^0 + 2^1 + 2^2 +.... 2^k\n",
    "    \n",
    "r = b/a = 2/1 = 2\n",
    "\n",
    "Sum = a(r^n - 1) / (r - 1) = 1 (2^n - 1) / (2-1) = 2^n - 1\n",
    "\n",
    "Therefore T(n) = O(2^n), i.e, Exponential time complexity\n",
    "\n",
    "\n",
    "\n",
    "b. T(n) = 2T(n/2) + n\n",
    "   T(n) = T(n/2) + T(n/2) + n\n",
    "    \n",
    "                n --- n\n",
    "               / \\\n",
    "              /   \\\n",
    "             /     \\\n",
    "            n/2    n/2 - n\n",
    "            /\\     /   \\\n",
    "           /  \\  n/4 n/4  - n  \n",
    "         n/4  n/4\n",
    "        \n",
    "        \n",
    "Continuing till k times\n",
    "\n",
    "Assuming n/2^k = 1, n = 2^k => log2(n) = k\n",
    "\n",
    "Adding the n at all the levels, we get\n",
    "O(n.k) = O(n.log n)\n",
    "\n"
   ]
  }
 ],
 "metadata": {
  "kernelspec": {
   "display_name": "Python 3 (ipykernel)",
   "language": "python",
   "name": "python3"
  },
  "language_info": {
   "codemirror_mode": {
    "name": "ipython",
    "version": 3
   },
   "file_extension": ".py",
   "mimetype": "text/x-python",
   "name": "python",
   "nbconvert_exporter": "python",
   "pygments_lexer": "ipython3",
   "version": "3.10.8"
  }
 },
 "nbformat": 4,
 "nbformat_minor": 5
}
